generational/spec/GC.Gen.HeapInvariant.fsti
@@ -76,6 +76,7 @@ val major_heap_shape_intro (major: heap) (fp: U64.t)
                     SweepInv.fp_valid fp major /\
                     Sweep.fp_in_heap fp major /\
                     Mark.no_black_objects major /\
+                    SweepInv.no_gray_objects major /\
                     Mark.no_pointer_to_blue major /\
                     no_scan_invariant major)
           (ensures major_heap_shape major fp)
@@ -93,6 +94,7 @@ val major_heap_shape_elim (major: heap) (fp: U64.t)
                    SweepInv.fp_valid fp major /\
                    Sweep.fp_in_heap fp major /\
                    Mark.no_black_objects major /\
+                   SweepInv.no_gray_objects major /\
                    Mark.no_pointer_to_blue major /\
                    no_scan_invariant major)
 
